tuned defs of sec_xyz

src/HOL/IMP/Sec_Type_Expr.thy
@@ -7,23 +7,46 @@ subsection "Security Levels and Expressions"
 
 type_synonym level = nat
 
+class sec =
+fixes sec :: "'a \<Rightarrow> nat"
+
 text{* The security/confidentiality level of each variable is globally fixed
 for simplicity. For the sake of examples --- the general theory does not rely
 on it! --- a variable of length @{text n} has security level @{text n}: *}
 
-definition sec :: "vname \<Rightarrow> level" where 
-  "sec n = size n"
+instantiation list :: (type)sec
+begin
+
+definition "sec(x :: 'a list) = length x"
+
+instance ..
+
+end
+
+instantiation aexp :: sec
+begin
 
 fun sec_aexp :: "aexp \<Rightarrow> level" where
-"sec_aexp (N n) = 0" |
-"sec_aexp (V x) = sec x" |
-"sec_aexp (Plus a\<^isub>1 a\<^isub>2) = max (sec_aexp a\<^isub>1) (sec_aexp a\<^isub>2)"
+"sec (N n) = 0" |
+"sec (V x) = sec x" |
+"sec (Plus a\<^isub>1 a\<^isub>2) = max (sec a\<^isub>1) (sec a\<^isub>2)"
+
+instance ..
+
+end
+
+instantiation bexp :: sec
+begin
 
 fun sec_bexp :: "bexp \<Rightarrow> level" where
-"sec_bexp (Bc v) = 0" |
-"sec_bexp (Not b) = sec_bexp b" |
-"sec_bexp (And b\<^isub>1 b\<^isub>2) = max (sec_bexp b\<^isub>1) (sec_bexp b\<^isub>2)" |
-"sec_bexp (Less a\<^isub>1 a\<^isub>2) = max (sec_aexp a\<^isub>1) (sec_aexp a\<^isub>2)"
+"sec (Bc v) = 0" |
+"sec (Not b) = sec b" |
+"sec (And b\<^isub>1 b\<^isub>2) = max (sec b\<^isub>1) (sec b\<^isub>2)" |
+"sec (Less a\<^isub>1 a\<^isub>2) = max (sec a\<^isub>1) (sec a\<^isub>2)"
+
+instance ..
+
+end
 
 
 abbreviation eq_le :: "state \<Rightarrow> state \<Rightarrow> level \<Rightarrow> bool"
@@ -35,11 +58,11 @@ abbreviation eq_less :: "state \<Rightarrow> state \<Rightarrow> level \<Rightar
 "s = s' (< l) == (\<forall> x. sec x < l \<longrightarrow> s x = s' x)"
 
 lemma aval_eq_if_eq_le:
-  "\<lbrakk> s\<^isub>1 = s\<^isub>2 (\<le> l);  sec_aexp a \<le> l \<rbrakk> \<Longrightarrow> aval a s\<^isub>1 = aval a s\<^isub>2"
+  "\<lbrakk> s\<^isub>1 = s\<^isub>2 (\<le> l);  sec a \<le> l \<rbrakk> \<Longrightarrow> aval a s\<^isub>1 = aval a s\<^isub>2"
 by (induct a) auto
 
 lemma bval_eq_if_eq_le:
-  "\<lbrakk> s\<^isub>1 = s\<^isub>2 (\<le> l);  sec_bexp b \<le> l \<rbrakk> \<Longrightarrow> bval b s\<^isub>1 = bval b s\<^isub>2"
+  "\<lbrakk> s\<^isub>1 = s\<^isub>2 (\<le> l);  sec b \<le> l \<rbrakk> \<Longrightarrow> bval b s\<^isub>1 = bval b s\<^isub>2"
 by (induct b) (auto simp add: aval_eq_if_eq_le)
 
 end
