src/HOL/IMP/Sec_Typing.thy
@@ -9,13 +9,13 @@ inductive sec_type :: "nat \<Rightarrow> com \<Rightarrow> bool" ("(_/ \<turnsti
 Skip:
   "l \<turnstile> SKIP" |
 Assign:
-  "\<lbrakk> sec x \<ge> sec_aexp a;  sec x \<ge> l \<rbrakk> \<Longrightarrow> l \<turnstile> x ::= a" |
+  "\<lbrakk> sec x \<ge> sec a;  sec x \<ge> l \<rbrakk> \<Longrightarrow> l \<turnstile> x ::= a" |
 Seq:
   "\<lbrakk> l \<turnstile> c\<^isub>1;  l \<turnstile> c\<^isub>2 \<rbrakk> \<Longrightarrow> l \<turnstile> c\<^isub>1;c\<^isub>2" |
 If:
-  "\<lbrakk> max (sec_bexp b) l \<turnstile> c\<^isub>1;  max (sec_bexp b) l \<turnstile> c\<^isub>2 \<rbrakk> \<Longrightarrow> l \<turnstile> IF b THEN c\<^isub>1 ELSE c\<^isub>2" |
+  "\<lbrakk> max (sec b) l \<turnstile> c\<^isub>1;  max (sec b) l \<turnstile> c\<^isub>2 \<rbrakk> \<Longrightarrow> l \<turnstile> IF b THEN c\<^isub>1 ELSE c\<^isub>2" |
 While:
-  "max (sec_bexp b) l \<turnstile> c \<Longrightarrow> l \<turnstile> WHILE b DO c"
+  "max (sec b) l \<turnstile> c \<Longrightarrow> l \<turnstile> WHILE b DO c"
 
 code_pred (expected_modes: i => i => bool) sec_type .
 
@@ -47,19 +47,19 @@ next
   case Seq thus ?case by auto
 next
   case (IfTrue b s c1)
-  hence "max (sec_bexp b) l \<turnstile> c1" by auto
+  hence "max (sec b) l \<turnstile> c1" by auto
   hence "l \<turnstile> c1" by (metis le_maxI2 anti_mono)
   thus ?case using IfTrue.IH by metis
 next
   case (IfFalse b s c2)
-  hence "max (sec_bexp b) l \<turnstile> c2" by auto
+  hence "max (sec b) l \<turnstile> c2" by auto
   hence "l \<turnstile> c2" by (metis le_maxI2 anti_mono)
   thus ?case using IfFalse.IH by metis
 next
   case WhileFalse thus ?case by auto
 next
   case (WhileTrue b s1 c)
-  hence "max (sec_bexp b) l \<turnstile> c" by auto
+  hence "max (sec b) l \<turnstile> c" by auto
   hence "l \<turnstile> c" by (metis le_maxI2 anti_mono)
   thus ?case using WhileTrue by metis
 qed
@@ -73,11 +73,11 @@ proof(induction arbitrary: t t' rule: big_step_induct)
 next
   case (Assign x a s)
   have [simp]: "t' = t(x := aval a t)" using Assign by auto
-  have "sec x >= sec_aexp a" using `0 \<turnstile> x ::= a` by auto
+  have "sec x >= sec a" using `0 \<turnstile> x ::= a` by auto
   show ?case
   proof auto
     assume "sec x \<le> l"
-    with `sec x >= sec_aexp a` have "sec_aexp a \<le> l" by arith
+    with `sec x >= sec a` have "sec a \<le> l" by arith
     thus "aval a s = aval a t"
       by (rule aval_eq_if_eq_le[OF `s = t (\<le> l)`])
   next
@@ -88,86 +88,86 @@ next
   case Seq thus ?case by blast
 next
   case (IfTrue b s c1 s' c2)
-  have "sec_bexp b \<turnstile> c1" "sec_bexp b \<turnstile> c2" using IfTrue.prems(2) by auto
+  have "sec b \<turnstile> c1" "sec b \<turnstile> c2" using IfTrue.prems(2) by auto
   show ?case
   proof cases
-    assume "sec_bexp b \<le> l"
-    hence "s = t (\<le> sec_bexp b)" using `s = t (\<le> l)` by auto
+    assume "sec b \<le> l"
+    hence "s = t (\<le> sec b)" using `s = t (\<le> l)` by auto
     hence "bval b t" using `bval b s` by(simp add: bval_eq_if_eq_le)
-    with IfTrue.IH IfTrue.prems(1,3) `sec_bexp b \<turnstile> c1`  anti_mono
+    with IfTrue.IH IfTrue.prems(1,3) `sec b \<turnstile> c1`  anti_mono
     show ?thesis by auto
   next
-    assume "\<not> sec_bexp b \<le> l"
-    have 1: "sec_bexp b \<turnstile> IF b THEN c1 ELSE c2"
-      by(rule sec_type.intros)(simp_all add: `sec_bexp b \<turnstile> c1` `sec_bexp b \<turnstile> c2`)
-    from confinement[OF IfTrue.hyps(2) `sec_bexp b \<turnstile> c1`] `\<not> sec_bexp b \<le> l`
+    assume "\<not> sec b \<le> l"
+    have 1: "sec b \<turnstile> IF b THEN c1 ELSE c2"
+      by(rule sec_type.intros)(simp_all add: `sec b \<turnstile> c1` `sec b \<turnstile> c2`)
+    from confinement[OF IfTrue.hyps(2) `sec b \<turnstile> c1`] `\<not> sec b \<le> l`
     have "s = s' (\<le> l)" by auto
     moreover
-    from confinement[OF IfTrue.prems(1) 1] `\<not> sec_bexp b \<le> l`
+    from confinement[OF IfTrue.prems(1) 1] `\<not> sec b \<le> l`
     have "t = t' (\<le> l)" by auto
     ultimately show "s' = t' (\<le> l)" using `s = t (\<le> l)` by auto
   qed
 next
   case (IfFalse b s c2 s' c1)
-  have "sec_bexp b \<turnstile> c1" "sec_bexp b \<turnstile> c2" using IfFalse.prems(2) by auto
+  have "sec b \<turnstile> c1" "sec b \<turnstile> c2" using IfFalse.prems(2) by auto
   show ?case
   proof cases
-    assume "sec_bexp b \<le> l"
-    hence "s = t (\<le> sec_bexp b)" using `s = t (\<le> l)` by auto
+    assume "sec b \<le> l"
+    hence "s = t (\<le> sec b)" using `s = t (\<le> l)` by auto
     hence "\<not> bval b t" using `\<not> bval b s` by(simp add: bval_eq_if_eq_le)
-    with IfFalse.IH IfFalse.prems(1,3) `sec_bexp b \<turnstile> c2` anti_mono
+    with IfFalse.IH IfFalse.prems(1,3) `sec b \<turnstile> c2` anti_mono
     show ?thesis by auto
   next
-    assume "\<not> sec_bexp b \<le> l"
-    have 1: "sec_bexp b \<turnstile> IF b THEN c1 ELSE c2"
-      by(rule sec_type.intros)(simp_all add: `sec_bexp b \<turnstile> c1` `sec_bexp b \<turnstile> c2`)
-    from confinement[OF big_step.IfFalse[OF IfFalse(1,2)] 1] `\<not> sec_bexp b \<le> l`
+    assume "\<not> sec b \<le> l"
+    have 1: "sec b \<turnstile> IF b THEN c1 ELSE c2"
+      by(rule sec_type.intros)(simp_all add: `sec b \<turnstile> c1` `sec b \<turnstile> c2`)
+    from confinement[OF big_step.IfFalse[OF IfFalse(1,2)] 1] `\<not> sec b \<le> l`
     have "s = s' (\<le> l)" by auto
     moreover
-    from confinement[OF IfFalse.prems(1) 1] `\<not> sec_bexp b \<le> l`
+    from confinement[OF IfFalse.prems(1) 1] `\<not> sec b \<le> l`
     have "t = t' (\<le> l)" by auto
     ultimately show "s' = t' (\<le> l)" using `s = t (\<le> l)` by auto
   qed
 next
   case (WhileFalse b s c)
-  have "sec_bexp b \<turnstile> c" using WhileFalse.prems(2) by auto
+  have "sec b \<turnstile> c" using WhileFalse.prems(2) by auto
   show ?case
   proof cases
-    assume "sec_bexp b \<le> l"
-    hence "s = t (\<le> sec_bexp b)" using `s = t (\<le> l)` by auto
+    assume "sec b \<le> l"
+    hence "s = t (\<le> sec b)" using `s = t (\<le> l)` by auto
     hence "\<not> bval b t" using `\<not> bval b s` by(simp add: bval_eq_if_eq_le)
     with WhileFalse.prems(1,3) show ?thesis by auto
   next
-    assume "\<not> sec_bexp b \<le> l"
-    have 1: "sec_bexp b \<turnstile> WHILE b DO c"
-      by(rule sec_type.intros)(simp_all add: `sec_bexp b \<turnstile> c`)
-    from confinement[OF WhileFalse.prems(1) 1] `\<not> sec_bexp b \<le> l`
+    assume "\<not> sec b \<le> l"
+    have 1: "sec b \<turnstile> WHILE b DO c"
+      by(rule sec_type.intros)(simp_all add: `sec b \<turnstile> c`)
+    from confinement[OF WhileFalse.prems(1) 1] `\<not> sec b \<le> l`
     have "t = t' (\<le> l)" by auto
     thus "s = t' (\<le> l)" using `s = t (\<le> l)` by auto
   qed
 next
   case (WhileTrue b s1 c s2 s3 t1 t3)
   let ?w = "WHILE b DO c"
-  have "sec_bexp b \<turnstile> c" using WhileTrue.prems(2) by auto
+  have "sec b \<turnstile> c" using WhileTrue.prems(2) by auto
   show ?case
   proof cases
-    assume "sec_bexp b \<le> l"
-    hence "s1 = t1 (\<le> sec_bexp b)" using `s1 = t1 (\<le> l)` by auto
+    assume "sec b \<le> l"
+    hence "s1 = t1 (\<le> sec b)" using `s1 = t1 (\<le> l)` by auto
     hence "bval b t1"
       using `bval b s1` by(simp add: bval_eq_if_eq_le)
     then obtain t2 where "(c,t1) \<Rightarrow> t2" "(?w,t2) \<Rightarrow> t3"
       using `(?w,t1) \<Rightarrow> t3` by auto
     from WhileTrue.IH(2)[OF `(?w,t2) \<Rightarrow> t3` `0 \<turnstile> ?w`
-      WhileTrue.IH(1)[OF `(c,t1) \<Rightarrow> t2` anti_mono[OF `sec_bexp b \<turnstile> c`]
+      WhileTrue.IH(1)[OF `(c,t1) \<Rightarrow> t2` anti_mono[OF `sec b \<turnstile> c`]
         `s1 = t1 (\<le> l)`]]
     show ?thesis by simp
   next
-    assume "\<not> sec_bexp b \<le> l"
-    have 1: "sec_bexp b \<turnstile> ?w" by(rule sec_type.intros)(simp_all add: `sec_bexp b \<turnstile> c`)
-    from confinement[OF big_step.WhileTrue[OF WhileTrue.hyps] 1] `\<not> sec_bexp b \<le> l`
+    assume "\<not> sec b \<le> l"
+    have 1: "sec b \<turnstile> ?w" by(rule sec_type.intros)(simp_all add: `sec b \<turnstile> c`)
+    from confinement[OF big_step.WhileTrue[OF WhileTrue.hyps] 1] `\<not> sec b \<le> l`
     have "s1 = s3 (\<le> l)" by auto
     moreover
-    from confinement[OF WhileTrue.prems(1) 1] `\<not> sec_bexp b \<le> l`
+    from confinement[OF WhileTrue.prems(1) 1] `\<not> sec b \<le> l`
     have "t1 = t3 (\<le> l)" by auto
     ultimately show "s3 = t3 (\<le> l)" using `s1 = t1 (\<le> l)` by auto
   qed
@@ -185,13 +185,13 @@ inductive sec_type' :: "nat \<Rightarrow> com \<Rightarrow> bool" ("(_/ \<turnst
 Skip':
   "l \<turnstile>' SKIP" |
 Assign':
-  "\<lbrakk> sec x \<ge> sec_aexp a; sec x \<ge> l \<rbrakk> \<Longrightarrow> l \<turnstile>' x ::= a" |
+  "\<lbrakk> sec x \<ge> sec a; sec x \<ge> l \<rbrakk> \<Longrightarrow> l \<turnstile>' x ::= a" |
 Seq':
   "\<lbrakk> l \<turnstile>' c\<^isub>1;  l \<turnstile>' c\<^isub>2 \<rbrakk> \<Longrightarrow> l \<turnstile>' c\<^isub>1;c\<^isub>2" |
 If':
-  "\<lbrakk> sec_bexp b \<le> l;  l \<turnstile>' c\<^isub>1;  l \<turnstile>' c\<^isub>2 \<rbrakk> \<Longrightarrow> l \<turnstile>' IF b THEN c\<^isub>1 ELSE c\<^isub>2" |
+  "\<lbrakk> sec b \<le> l;  l \<turnstile>' c\<^isub>1;  l \<turnstile>' c\<^isub>2 \<rbrakk> \<Longrightarrow> l \<turnstile>' IF b THEN c\<^isub>1 ELSE c\<^isub>2" |
 While':
-  "\<lbrakk> sec_bexp b \<le> l;  l \<turnstile>' c \<rbrakk> \<Longrightarrow> l \<turnstile>' WHILE b DO c" |
+  "\<lbrakk> sec b \<le> l;  l \<turnstile>' c \<rbrakk> \<Longrightarrow> l \<turnstile>' WHILE b DO c" |
 anti_mono':
   "\<lbrakk> l \<turnstile>' c;  l' \<le> l \<rbrakk> \<Longrightarrow> l' \<turnstile>' c"
 
@@ -219,14 +219,14 @@ inductive sec_type2 :: "com \<Rightarrow> level \<Rightarrow> bool" ("(\<turnsti
 Skip2:
   "\<turnstile> SKIP : l" |
 Assign2:
-  "sec x \<ge> sec_aexp a \<Longrightarrow> \<turnstile> x ::= a : sec x" |
+  "sec x \<ge> sec a \<Longrightarrow> \<turnstile> x ::= a : sec x" |
 Seq2:
   "\<lbrakk> \<turnstile> c\<^isub>1 : l\<^isub>1;  \<turnstile> c\<^isub>2 : l\<^isub>2 \<rbrakk> \<Longrightarrow> \<turnstile> c\<^isub>1;c\<^isub>2 : min l\<^isub>1 l\<^isub>2 " |
 If2:
-  "\<lbrakk> sec_bexp b \<le> min l\<^isub>1 l\<^isub>2;  \<turnstile> c\<^isub>1 : l\<^isub>1;  \<turnstile> c\<^isub>2 : l\<^isub>2 \<rbrakk>
+  "\<lbrakk> sec b \<le> min l\<^isub>1 l\<^isub>2;  \<turnstile> c\<^isub>1 : l\<^isub>1;  \<turnstile> c\<^isub>2 : l\<^isub>2 \<rbrakk>
   \<Longrightarrow> \<turnstile> IF b THEN c\<^isub>1 ELSE c\<^isub>2 : min l\<^isub>1 l\<^isub>2" |
 While2:
-  "\<lbrakk> sec_bexp b \<le> l;  \<turnstile> c : l \<rbrakk> \<Longrightarrow> \<turnstile> WHILE b DO c : l"
+  "\<lbrakk> sec b \<le> l;  \<turnstile> c : l \<rbrakk> \<Longrightarrow> \<turnstile> WHILE b DO c : l"
 
 
 lemma sec_type2_sec_type': "\<turnstile> c : l \<Longrightarrow> l \<turnstile>' c"
